refactor

src/theories/lang.v
@@ -3,118 +3,118 @@ From stdpp Require Import gmap fin_maps list binders strings countable fin mapse
 From iris.prelude Require Import options.
 From iris.algebra Require Import ofe.
 From iris.program_logic Require Import language ectx_language ectxi_language.
-From ExtLib Require Import Structures.Monads.
-Require Import monad_aux.
-Require Import machine_base.
+From hypvis Require Import machine monad.
 
-Export monad_notation.
+Import MonadNotation.
+Import Option.
 Open Scope monad_scope.
 
 Context `(HypervisorParams : HypervisorParameters).
 
 (* State *)
 
-Definition Mem : Type :=
-  gmap Addr Word.
+Definition mem : Type :=
+  gmap addr word.
 
-Definition RegFile : Type :=
-  gmap RegName Word.
+Definition reg_file : Type :=
+  gmap reg_name word.
 
-Definition VMID : Type :=
-  fin VMCount.
+Definition vmid : Type :=
+  fin vm_count.
 
-Definition PID : Type :=
-  fin PageCount.
+Definition pid : Type :=
+  fin page_count.
 
-Definition PageTable : Type :=
-  gmap PID Perm.
+Definition page_table : Type :=
+  gmap pid permission.
 
-Definition TXBuffer : Type :=
-  PID.
+Definition tx_buffer : Type :=
+  pid.
 
-Definition RXBuffer : Type :=
-  (PID * option(VMID)).
+Definition rx_buffer : Type :=
+  (pid * option vmid).
 
-Definition MailBox : Type :=
-  (TXBuffer * RXBuffer).
+Definition mail_box : Type :=
+  (tx_buffer * rx_buffer).
 
-Definition CurrentVM := VMID.
+Definition current_vm := vmid.
 
-Definition VMState : Type :=
-  gmap VMID (RegFile * MailBox * PageTable).
+Definition vm_states : Type :=
+  gmap vmid (reg_file * mail_box * page_table).
 
-Definition Flag : Type :=
-  bool.
+Definition transaction : Type :=
+  vmid (* sender *)
+  * word (*flag *)
+  * word (* tag *)
+  * gmap vmid (gmap pid bool)
+  * transaction_type.
 
-Definition Transaction : Type :=
-  VMID (* sender *) * Word (*flag *) * Word (* tag *) * gmap VMID (gmap PID Flag) * TransactionType.
+Definition handle := word.
 
-Definition Handle := Word.
+Definition transactions : Type :=
+  gmap handle transaction.
 
-Definition Transactions : Type :=
-  gmap Handle Transaction.
-
-Definition State : Type :=
-  VMState * CurrentVM * Mem * Transactions.
+Definition state : Type :=
+  vm_states * current_vm * mem * transactions.
 
 (* Getters *)
 
-Definition vmStates (st : State) : VMState :=
+Definition get_vm_states (st : state) : vm_states :=
   fst (fst (fst st)).
 
-Definition currentVM (st : State) : CurrentVM :=
+Definition get_current_vm (st : state) : current_vm :=
   snd (fst (fst st)).
 
-Definition mem (st : State) : Mem :=
+Definition get_mem (st : state) : mem :=
   snd (fst st).
 
-Definition transactions (st : State) : Transactions :=
+Definition get_transactions (st : state) : transactions :=
   snd st.
 
-Definition vmState (st : State) (v : VMID) : option (RegFile * MailBox * PageTable) :=
-  (vmStates st) !! v.
+Definition get_vm_state (st : state) (v : vmid) : option (reg_file * mail_box * page_table) :=
+  (get_vm_states st) !! v.
 
-Definition vmRegFile (st : State) (v : VMID) : option RegFile :=
-  match vmState st v with
+Definition get_vm_reg_file (st : state) (v : vmid) : option reg_file :=
+  match get_vm_state st v with
   | None => None
   | Some a => Some (fst (fst a))
   end.
 
-Definition vmMailBox (st : State) (v : VMID) : option MailBox :=
-  match vmState st v with
+Definition get_vm_mail_box (st : state) (v : vmid) : option mail_box :=
+  match get_vm_state st v with
   | None => None
   | Some a => Some (snd (fst a))
   end.
 
-Definition vmPageTable (st : State) (v : VMID) : option PageTable :=
-  match vmState st v with
+Definition get_vm_page_table (st : state) (v : vmid) : option page_table :=
+  match get_vm_state st v with
   | None => None
   | Some a => Some (snd a)
   end.
 
 (* Conf *)
 
-Inductive ExecMode : Type :=
+Inductive exec_mode : Type :=
 | ExecI
 | NextI
 | HaltI
 | FailI.
 
-Inductive ControlMode : Type :=
-| YieldM : VMID -> ControlMode
+Inductive control_mode : Type :=
+| YieldM : vmid -> control_mode
 | NormalM.
 
-Definition Conf : Type := ExecMode * State.
+Definition conf : Type := exec_mode * state.
 
 (* Aux funcs *)
 
-Definition checkPermPage (st : State) (v : VMID) (pid : PID) (p : Perm) : bool :=
-  match (vmPageTable st v) with
+Definition check_perm_page (st : state) (v : vmid) (p : pid) (pm : permission) : bool :=
+  match (get_vm_page_table st v) with
   | None => false
   | Some pt =>
-    match pt !! pid with
+    match pt !! p with
     | Some p' =>
-      match (decide (p = p')) with
+      match (decide (pm = p')) with
       | left _ => true
       | right _ => false
       end
@@ -122,133 +122,122 @@ Definition checkPermPage (st : State) (v : VMID) (pid : PID) (p : Perm) : bool :
     end
   end.
 
-Definition checkPermAddr (st : State) (v : VMID) (addr : Addr) (p : Perm) : bool :=
-  checkPermPage st v (MMTranslation addr) p.
+Definition check_perm_addr (st : state) (v : vmid) (a : addr) (p : permission) : bool :=
+  check_perm_page st v (mm_translation a) p.
 
-Definition checkAccessPage (st : State) (v : VMID) (pid : PID) : bool :=
-  match (vmPageTable st v) with
+Definition check_access_page (st : state) (v : vmid) (p : pid) : bool :=
+  match get_vm_page_table st v with
   | None => false
   | Some pt =>
-    match pt !! pid with
-    | Some p => isAccessible p
+    match pt !! p with
+    | Some p' => is_accessible p'
     | _ => false
     end
   end.
 
-Definition checkAccessAddr (st : State) (v : VMID) (addr : Addr) : bool :=
-  checkAccessPage st v (MMTranslation addr).
+Definition check_access_addr (st : state) (v : vmid) (a : addr) : bool :=
+  check_access_page st v (mm_translation a).
 
-Definition checkOwnershipPage (st : State) (v : VMID) (pid : PID) : bool :=
-  match (vmPageTable st v) with
+Definition check_ownership_page (st : state) (v : vmid) (p : pid) : bool :=
+  match get_vm_page_table st v with
   | None => false
   | Some pt =>
-    match pt !! pid with
-    | Some p => isOwned p
+    match pt !! p with
+    | Some p' => is_owned p'
     | _ => false
     end
   end.
 
-Definition checkOwnershipAddr (st : State) (v : VMID) (addr : Addr) : bool :=
-  checkOwnershipPage st v (MMTranslation addr).
+Definition check_ownership_addr (st : state) (v : vmid) (a : addr) : bool :=
+  check_ownership_page st v (mm_translation a).
 
-Definition updateGeneralRegGlobal (st : State) (v : VMID) (r : RegName) (w : Word) : option State :=
+Definition update_general_reg_global (st : state) (v : vmid) (r : reg_name) (w : word) : option state :=
   match r with
   | PC => None
   | NZ => None
   | R n fin =>
-    match vmState st v with
+    match get_vm_state st v with
     | None => None
     | Some (rf, mb, pt) =>
-      Some (<[v:=(<[r:=w]>rf, mb, pt)]>(vmStates st),
-            currentVM st,
-            mem st, transactions st)
+      Some (<[v:=(<[r:=w]>rf, mb, pt)]>(get_vm_states st),
+            get_current_vm st,
+            get_mem st, get_transactions st)
     end
   end.
 
-Definition updateGeneralReg (st : State) (r : RegName) (w : Word) : option State :=
-  updateGeneralRegGlobal st (currentVM st) r w.
+Definition update_general_reg (st : state) (r : reg_name) (w : word) : option state :=
+  update_general_reg_global st (get_current_vm st) r w.
 
-Definition updateSysRegGlobal (st : State) (v : VMID) (r : RegName) (w : Word) : option State :=
+Definition update_sys_reg_global (st : state) (v : vmid) (r : reg_name) (w : word) : option state :=
   match r with
   | R n fin => None
-  | _ => match vmState st v with
+  | _ => match get_vm_state st v with
          | None => None
          | Some (rf, mb, pt) =>
-           Some (<[v:=(<[r:=w]>rf, mb, pt)]>(vmStates st),
-                 currentVM st,
-                 mem st, transactions st)
+           Some (<[v:=(<[r:=w]>rf, mb, pt)]>(get_vm_states st),
+                 get_current_vm st,
+                 get_mem st, get_transactions st)
          end
   end.
 
-Definition updateSysReg (st : State) (r : RegName) (w : Word) : option State :=
-  updateSysRegGlobal st (currentVM st) r w.
+Definition update_sys_reg (st : state) (r : reg_name) (w : word) : option state :=
+  update_sys_reg_global st (get_current_vm st) r w.
 
-Definition getRegGlobal (st : State) (v : VMID) (r : RegName) : option Word :=
-  match vmRegFile st v with
+Definition get_reg_global (st : state) (v : vmid) (r : reg_name) : option word :=
+  match get_vm_reg_file st v with
   | None => None
   | Some rf => rf !! r 
   end.
 
-Definition getReg (st : State) (r : RegName) : option Word :=
-  getRegGlobal st (currentVM st) r.
+Definition get_reg (st : state) (r : reg_name) : option word :=
+  get_reg_global st (get_current_vm st) r.
 
-Definition updatePageTableGlobal (st : State) (v : VMID) (pid : PID) (p : Perm) : option State :=
-  match vmState st v with
+Definition update_page_table_global (st : state) (v : vmid) (p : pid) (pm : permission) : option state :=
+  match get_vm_state st v with
   | None => None
   | Some (rf, mb, pt) =>
-    Some (<[v:=(rf, mb, <[pid:=p]>pt)]>(vmStates st),
-          currentVM st,
-          mem st, transactions st)
+    Some (<[v:=(rf, mb, <[p:=pm]>pt)]>(get_vm_states st),
+          get_current_vm st,
+          get_mem st, get_transactions st)
   end.
 
-Definition updatePageTable (st : State) (pid : PID) (p : Perm) : option State :=
-  updatePageTableGlobal st (currentVM st) pid p.
+Definition update_page_table (st : state) (p : pid) (pm : permission) : option state :=
+  update_page_table_global st (get_current_vm st) p pm.
 
-Definition getPageTableGlobal (st : State) (v : VMID) (pid : PID) : option Perm :=
-  match vmPageTable st v with
+Definition get_page_table_global (st : state) (v : vmid) (p : pid) : option permission :=
+  match get_vm_page_table st v with
   | None => None
-  | Some pt => pt !! pid
+  | Some pt => pt !! p
   end.
 
-Definition getPageTable (st : State) (pid : PID) : option Perm :=
-  getPageTableGlobal st (currentVM st) pid.
+Definition get_page_table (st : state) (p : pid) : option permission :=
+  get_page_table_global st (get_current_vm st) p.
                 
-Definition updateMemUnsafe (st : State) (a : Addr) (w : Word) : State :=
-  (vmStates st, currentVM st, <[a:=w]>(mem st), transactions st).
+Definition update_memory_unsafe (st : state) (a : addr) (w : word) : state :=
+  (get_vm_states st, get_current_vm st, <[a:=w]>(get_mem st), get_transactions st).
 
-Definition updateMem (st : State) (a : Addr) (w : Word) : option State :=
-  if checkAccessAddr st (currentVM st) a
-  then ret (updateMemUnsafe st a w)
+Definition update_memory (st : state) (a : addr) (w : word) : option state :=
+  if check_access_addr st (get_current_vm st) a
+  then unit (update_memory_unsafe st a w)
   else None.
 
-Definition getMemUnsafe (st : State) (a : Addr) : option Word :=
-  (mem st) !! a.
+Definition get_memory_unsafe (st : state) (a : addr) : option word :=
+  (get_mem st) !! a.
 
-Definition getMem (st : State) (a : Addr) : option Word :=
-  if checkAccessAddr st (currentVM st) a
-  then getMemUnsafe st a
+Definition get_memory (st : state) (a : addr) : option word :=
+  if check_access_addr st (get_current_vm st) a
+  then get_memory_unsafe st a
   else None.
-(* 
-Definition writeTXUnsafe (st : State) (v : VMID) (msg : vec Word PageCount) : option State :=
-  match vmState st v with
-  | None => None
-  | Some (rf, (txPid, _), pt) => ret (updateMemUnsafe st txAddr msg)
-  end.
 
-Definition writeTX (st : State) (v : VMID) (msg : Word) : option State :=
-    match vmState st v with
-  | None => None
-  | Some (rf, (txAddr, _), pt) => updateMem st txAddr msg
-  end.
- *)
-Lemma atLeastOneAddrInPage (pid : PID) : vec Word (S (PageSize - 1)).
+(* ! depends on a constant ! *)
+Lemma at_least_one_addr_in_page (p : pid) : vec word (S (page_size - 1)).
 Proof.
-  pose proof PageSizeSanity as H.
-  pose proof WordSizeAtLeast as H'.
-  pose proof (MMTranslationInv pid) as H''.
-  destruct PageSize.
+  pose proof page_size_sanity as H.
+  pose proof word_size_at_least as H'.
+  pose proof (mm_translation_inv p) as H''.
+  destruct page_size.
   - simpl in H. 
-    unfold WordSizeLowerBound in H'.
+    unfold word_size_lower_bound in H'.
     rewrite <- H in H'.
     exfalso.
     apply (Nat.nlt_0_r 15 H').
@@ -257,108 +246,109 @@ Proof.
     exact H''.
 Qed.
 
-Definition getTXBaseAddrGlobal (st : State) (v : VMID) : option Word :=
-  match vmState st v with
+Definition get_tx_base_addr_global (st : state) (v : vmid) : option word :=
+  match get_vm_state st v with
   | Some (rf, (pid, _), pt) =>
-    Some (@Vector.hd Word (PageSize - 1) (atLeastOneAddrInPage pid))
+    Some (@Vector.hd word (page_size - 1) (at_least_one_addr_in_page pid))
   | _ => None
   end.
 
-Definition isRXReadyGlobal (st : State) (v : VMID) : bool :=
-  match vmState st v with
+Definition is_rx_ready_global (st : state) (v : vmid) : bool :=
+  match get_vm_state st v with
   | Some (rf, (_, (_, Some _)), pt) => true
   | _ => false
   end.
 
-Definition isRXReady (st : State) : bool :=
-  isRXReadyGlobal st (currentVM st).
+Definition is_rx_ready (st : state) : bool :=
+  is_rx_ready_global st (get_current_vm st).
 
-Definition getRXSenderGlobal (st : State) (v : VMID) : option VMID :=
-  match vmState st v with
+Definition get_rx_sender_global (st : state) (v : vmid) : option vmid :=
+  match get_vm_state st v with
   | Some (rf, (_, (_, Some v')), pt) => Some v'
   | _ => None
   end.
 
-Definition getRXSender (st : State) : option VMID :=
-  getRXSenderGlobal st (currentVM st).
+Definition get_rx_sender (st : state) : option vmid :=
+  get_rx_sender_global st (get_current_vm st).
 
-Program Definition getRXBaseAddrGlobal (st : State) (v : VMID) : option Word :=
-  match vmState st v with
-  | Some (rf, (_, (pid, Some _)), pt) => Some (@Vector.hd Word (PageSize - 1) (atLeastOneAddrInPage pid))
+Definition get_rx_base_addr_global (st : state) (v : vmid) : option word :=
+  match get_vm_state st v with
+  | Some (rf, (_, (pid, Some _)), pt) => Some (@Vector.hd word (page_size - 1) (at_least_one_addr_in_page pid))
   | _ => None
   end.
 
-(*
-Definition getRXMsg (st : State) : option Word :=
-  match vmState st (currentVM st) with
-  | Some (rf, (_, (addr, Some _)), pt) => getMem st addr
-  | _ => None
-  end.
- *)
+Definition get_rx_base_addr (st : state) : option word :=
+  get_rx_base_addr_global st (get_current_vm st).
 
-Definition emptyRXGlobal (st : State) (v : VMID) : option State :=
-  match vmState st v with
+Definition empty_rx_global (st : state) (v : vmid) : option state :=
+  match get_vm_state st v with
   | Some (rf, (txAddr, (rxAddr, Some _)), pt) =>
-    Some (<[v:=(rf, (txAddr, (rxAddr, None)), pt)]>(vmStates st),
-          currentVM st,
-          mem st, transactions st)
+    Some (<[v:=(rf, (txAddr, (rxAddr, None)), pt)]>(get_vm_states st),
+          get_current_vm st,
+          get_mem st, get_transactions st)
   | _ => None
   end.
-Definition emptyRX (st : State) : option State :=
-  emptyRXGlobal st (currentVM st).
 
-Definition copyFromAddrToAddrUnsafe (st : State) (src dst : Addr) : option State :=
-  w <- getMemUnsafe st src ;;;
-  Some (updateMemUnsafe st dst w).
+Definition empty_rx (st : state) : option state :=
+  empty_rx_global st (get_current_vm st).
 
-Definition copyPageUnsafe (st : State) (src dst : PID) : option State :=
-  let src' := MMTranslationInv src
-  in
-  let dst' := MMTranslationInv dst
-  in
-  let H := vzip_with (fun x y => (x, y)) src' dst'
-  in
-  monad_general.foldrMVec (fun x s => match x with | (a, b) => copyFromAddrToAddrUnsafe s a b end) H st.
+Definition copy_from_addr_to_addr_unsafe (st : state) (src dst : addr) : option state :=
+  w <- get_memory_unsafe st src ;;;
+  Some (update_memory_unsafe st dst w).
 
-Definition transferMsgUnsafe (st : State) (v : VMID) (r : VMID) : option State :=
-  match vmState st v with
+Definition copy_page_unsafe (st : state) (src dst : pid) : option state :=
+  foldr (fun x s =>
+           match x with
+           | (a, b) =>
+             (@bind option _ state state s (fun y => copy_from_addr_to_addr_unsafe y a b))
+           end)
+        (Some st)
+        (vzip_with (fun x y => (x, y)) (mm_translation_inv src) (mm_translation_inv dst)).
+
+Definition transfer_msg_unsafe (st : state) (v : vmid) (r : vmid) : option state :=
+  match get_vm_state st v with
   | Some (_, (txPid, _), _) =>
-    match vmState st r with
+    match get_vm_state st r with
     | Some (rf, (_, (rxPid, _)), pt) =>
-      copyPageUnsafe st txPid rxPid
+      copy_page_unsafe st txPid rxPid
     | _ => None
     end
   | _ => None
   end.
 
-Definition tryIncrWord (n : Word) (p : nat) : option Word :=
-  match (nat_lt_dec (n + p) WordSize) with
+Definition transfer_msg (st : state) (r : vmid) : option state :=
+  transfer_msg_unsafe st (get_current_vm st) r.
+
+Definition try_incr_word (n : word) (p : nat) : option word :=
+  match (nat_lt_dec (n + p) word_size) with
   | left l => Some (@nat_to_fin (n + p) _ l)
   | _ => None
   end.
 
-Lemma finMax {n : nat} (x y : fin n) : fin n.
+Lemma fin_max {n : nat} (x y : fin n) : fin n.
 Proof.
   destruct (Fin.to_nat x);
     destruct (Fin.to_nat y);
     destruct (x <? y); auto.
 Defined.
 
-Definition freshHandleHelper (val : Handle) (acc : option Handle) : option Handle :=
-  match (tryIncrWord val 1) with
+Definition fresh_handle_helper (val : handle) (acc : option handle) : option handle :=
+  match (try_incr_word val 1) with
   | None => None
   | Some val' => match acc with
                  | None => Some val'
-                 | Some acc' => Some (finMax val' acc')
+                 | Some acc' => Some (fin_max val' acc')
                  end
   end.
 
-Definition freshHandle (m : gmap Handle Transaction) : option Handle := 
-  set_fold freshHandleHelper None (@dom (gmap Handle Transaction) (gset Handle) gset_dom m).
+(* TODO: pick the least *free* handle *)
+Definition fresh_handle (m : gmap handle transaction) : option handle := 
+  set_fold fresh_handle_helper None (@dom (gmap handle transaction) (gset handle) gset_dom m).
 
-Definition MemoryRegionDescriptor : Type :=
-  Word (* length *) * VMID (* receiver *) * list PID (* pids *).  
+Definition memory_region_descriptor : Type :=
+  word (* length *) * vmid (* receiver *) * list pid (* pids *).  
 
+(* It would make a lot of things simplier... *)
 (*
 Instance proofIrrelNoDup {A : Type} {l : list A} `{EqDecision A} : ProofIrrel (NoDup l).
 Proof.
@@ -405,465 +395,474 @@ Proof.
 Qed.
 *)
 
-Definition TransactionDescriptor : Type :=
-  VMID (* Sender *) * option Handle (* Handle *) * Word (* Tag *)
-  * Word (* Flag *)
-  * gmap VMID (listset_nodup PID) (* Receivers *).
+Definition transaction_descriptor : Type :=
+  vmid (* Sender *) * option handle (* Handle *) * word (* Tag *)
+  * word (* Flag *)
+  * gmap vmid (listset_nodup pid) (* Receivers *).
 
-Definition memoryRegionsToGmap (md : listset_nodup MemoryRegionDescriptor) : gmap VMID (listset_nodup PID) :=
+Definition memory_regions_to_gmap (md : listset_nodup memory_region_descriptor) : gmap vmid (listset_nodup pid) :=
   set_fold (fun v acc => match decide (NoDup (snd v)) with
                          | left l => map_insert (snd (fst v)) (ListsetNoDup v.2 l) acc
                          | right r => acc
                          end) empty md.
 
-Definition addrOffset (base : Addr) (offset : nat) : option Addr :=
-  tryIncrWord base offset.
+Definition addr_offset (base : addr) (offset : nat) : option addr :=
+  try_incr_word base offset.
 
-Definition getMemWithOffset (st : State) (base : Addr) (offset : nat) : option Word :=
-  addr <- addrOffset base offset ;;;
-  getMem st addr.
+Definition get_memory_with_offset (st : state) (base : addr) (offset : nat) : option word :=
+  addr <- addr_offset base offset ;;;
+  get_memory st addr.
 
-Definition parseMemoryRegionDescriptor (st : State) (base : Addr) : option MemoryRegionDescriptor :=
-  match getMemWithOffset st base 0 with
-  | None => None
-  | Some l =>
-    match getMemWithOffset st base 1 with
-    | None => None
-    | Some r =>
-      match DecodeVMID r with
-      | None => None
-      | Some r' =>
-        let ls := foldl (fun acc v => cons (bind (getMemWithOffset st base (2 + v)) DecodePID) acc) nil (seq 0 (fin_to_nat l))
-        in
-        match (monad_general.sequenceMList ls) with
-        | None => None
-        | Some ls' => ret (l, r', ls')
-        end
-      end
-    end
-  end.
+Definition parse_memory_region_descriptor (st : state) (base : addr) : option memory_region_descriptor :=
+  l <- get_memory_with_offset st base 0 ;;;
+  r <- get_memory_with_offset st base 1 ;;;
+  r' <- decode_vmid r ;;;
+  ls' <- sequence_a (foldl (fun acc v => cons (bind (get_memory_with_offset st base (2 + v)) decode_pid) acc) nil (seq 0 (fin_to_nat l))) ;;;
+  unit (l, r', ls').
 
-Definition parseMemoryRegionDescriptors (st : State) (base : Addr) (count : nat) : option (listset_nodup MemoryRegionDescriptor) :=
-  let ls := (foldl (fun acc v =>
-                     cons (bind (addrOffset base v) (parseMemoryRegionDescriptor st)) acc) (@nil (option MemoryRegionDescriptor)) (seq 0 count))
-  in
-  match monad_general.sequenceMList ls with
-  | None => None
-  | Some ls' =>
-    match NoDup_dec ls' with
-    | left prf => ret (ListsetNoDup ls' prf)
+Definition parse_memory_region_descriptors (st : state) (base : addr) (count : nat) : option (listset_nodup memory_region_descriptor) :=
+  ls' <- sequence_a (foldl (fun acc v =>
+                     cons (bind (addr_offset base v) (parse_memory_region_descriptor st)) acc) (@nil (option memory_region_descriptor)) (seq 0 count)) ;;;
+ (match NoDup_dec ls' with
+    | left prf => unit (ListsetNoDup ls' prf)
     | right prf => None
-    end
-  end.
+  end).
 
 (* TODO: Prop version, reflection *)
-Definition parseTransactionDescriptor (st : State) (wl : Word) (base : Addr) (ty : TransactionType) : option TransactionDescriptor :=
+Definition parse_transaction_descriptor (st : state) (wl : word) (base : addr) (ty : transaction_type) : option transaction_descriptor :=
   (* Main fields *)
-  vs <- getMemWithOffset st base 0 ;;;
-  vs' <- DecodeVMID vs ;;;
-  wf <- getMemWithOffset st base 1 ;;;
-  wh <- getMemWithOffset st base 2 ;;;
-  wt <- getMemWithOffset st base 3 ;;;
-  wc <- getMemWithOffset st base 4 ;;;
-  memDescrBase <- addrOffset base 5 ;;;
-  memDescrs <- parseMemoryRegionDescriptors st memDescrBase (fin_to_nat wc) ;;;
+  vs <- get_memory_with_offset st base 0 ;;;
+  vs' <- decode_vmid vs ;;;
+  wf <- get_memory_with_offset st base 1 ;;;
+  wh <- get_memory_with_offset st base 2 ;;;
+  wt <- get_memory_with_offset st base 3 ;;;
+  wc <- get_memory_with_offset st base 4 ;;;
+  memDescrBase <- addr_offset base 5 ;;;
+  memDescrs <- parse_memory_region_descriptors st memDescrBase (fin_to_nat wc) ;;;
   (* Validate length *)                                          
-  _ <- addrOffset base (fin_to_nat wl) ;;;
-  _ <- @monad_option.boolCheckOption True (negb (fin_to_nat wc =? 0)) ;;;
-  _ <- @monad_option.boolCheckOption True (fin_to_nat wl =? 5 + 3 * (fin_to_nat wc) + (set_fold (fun v acc => length (snd v) + acc) 0 memDescrs)) ;;;
-  _ <- @monad_option.boolCheckOption True (match ty with
+  _ <- addr_offset base (fin_to_nat wl) ;;;
+  _ <- @bool_check_option True (negb (fin_to_nat wc =? 0)) ;;;
+  _ <- @bool_check_option True (fin_to_nat wl =? 5 + 3 * (fin_to_nat wc) + (set_fold (fun v acc => length (snd v) + acc) 0 memDescrs)) ;;;
+  _ <- @bool_check_option True (match ty with
                                      | Donation => (fin_to_nat wc) =? 1
                                      | _ => true
                                      end) ;;;
-  ret (vs', (if (fin_to_nat wh) =? 0 then None else Some wh), wt, wf, memoryRegionsToGmap memDescrs).
+  unit (vs', (if (fin_to_nat wh) =? 0 then None else Some wh), wt, wf, memory_regions_to_gmap memDescrs).
                                                            
-Definition insertTransaction (st : State) (h : Handle) (t : Transaction) : State :=
-  (vmStates st, currentVM st, mem st, <[h:=t]>(transactions st)).
+Definition insert_transaction (st : state) (h : handle) (t : transaction) : state :=
+  (get_vm_states st, get_current_vm st, get_mem st, <[h:=t]>(get_transactions st)).
 
-Definition newTransaction (st : State) (vid : VMID)
-           (tt : TransactionType)
-           (flag tag : Word)
-           (m : gmap VMID (gmap PID Flag))  : option State :=
-  if map_fold (fun _ v acc => andb acc (set_fold (fun v' acc' => andb acc' (checkOwnershipPage st vid v')) true (@dom (gmap PID Flag) (gset PID) gset_dom v))) true m
+Definition new_transaction (st : state) (vid : vmid)
+           (tt : transaction_type)
+           (flag tag : word)
+           (m : gmap vmid (gmap pid bool))  : option state :=
+  if map_fold (fun _ v acc => andb acc (set_fold (fun v' acc' => andb acc' (check_ownership_page st vid v')) true (@dom (gmap pid bool) (gset pid) gset_dom v))) true m
   then
-    match freshHandle (transactions st) with
+    match fresh_handle (get_transactions st) with
     | None => None
     | Some h' =>
-      ret (insertTransaction st h' (vid, flag, tag, m, tt))
+      unit (insert_transaction st h' (vid, flag, tag, m, tt))
     end
   else None.
 
-Definition getTransaction (st : State) (h : Handle) : option Transaction :=
-  (transactions st) !! h.
+Definition get_transaction (st : state) (h : handle) : option transaction :=
+  (get_transactions st) !! h.
 
-Definition removeTransaction (s : State) (handle : Handle) : State :=
-  (vmStates s, currentVM s, mem s, delete handle (transactions s)).
+Definition remove_transaction (s : state) (h : handle) : state :=
+  (get_vm_states s, get_current_vm s, get_mem s, delete h (get_transactions s)).
 
-Definition newTransactionFromDescriptor (st : State) (ty : TransactionType) (td : TransactionDescriptor) : option State :=
+Definition new_transaction_from_descriptor (st : state) (ty : transaction_type) (td : transaction_descriptor) : option state :=
   match td with
-  | (s, None, t, f, rs) => newTransaction st s ty f t (fmap (fun x => set_to_map (fun el => (el, false)) x) rs)
+  | (s, None, t, f, rs) => new_transaction st s ty f t (base.fmap (fun x => set_to_map (fun el => (el, false)) x) rs)
   | _ => None
   end.
 
-Definition newTransactionFromDescriptorInTXUnsafe (st : State) (v : VMID) (wl : Word) (ty : TransactionType) : option State :=
-  if (PageSize <? fin_to_nat wl)
+Definition new_transaction_from_descriptor_in_tx_unsafe (st : state) (v : vmid) (wl : word) (ty : transaction_type) : option state :=
+  if (page_size <? fin_to_nat wl)
   then None
   else
-    txBAddr <- getTXBaseAddrGlobal st v ;;;
-    td <- parseTransactionDescriptor st wl txBAddr ty ;;;
-    newTransactionFromDescriptor st ty td.
+    txBAddr <- get_tx_base_addr_global st v ;;;
+    td <- parse_transaction_descriptor st wl txBAddr ty ;;;
+    new_transaction_from_descriptor st ty td.
 
-Definition updateOffsetPC (st : State) (dir : bool) (offset : nat) : option State :=
+Definition update_offset_PC (st : state) (dir : bool) (offset : nat) : option state :=
   bind
-    (vmRegFile st (currentVM st))
+    (get_vm_reg_file st (get_current_vm st))
     (fun rf =>
        bind (rf !! PC)
             (fun v =>
                let v' := fin_to_nat v in
                if dir
                then
-                 match (nat_lt_dec (v' + offset) WordSize) with
-                 | left l => updateSysReg st PC (@nat_to_fin (v' + offset) _ l)
+                 match (nat_lt_dec (v' + offset) word_size) with
+                 | left l => update_sys_reg st PC (@nat_to_fin (v' + offset) _ l)
                  | _ => None
                  end
                else
-                 match (nat_lt_dec (v' - offset) WordSize) with
-                 | left l => updateSysReg st PC (@nat_to_fin (v' - offset) _ l)
+                 match (nat_lt_dec (v' - offset) word_size) with
+                 | left l => update_sys_reg st PC (@nat_to_fin (v' - offset) _ l)
                  | _ => None
                  end
     )).
 
-Definition updateIncrPC (st : State) : option State :=
-  updateOffsetPC st true 2.
+Definition update_incr_PC (st : state) : option state :=
+  update_offset_PC st true 2.
 
-Definition updateCurrentVMID (st : State) (v : VMID) : State :=
-  (vmStates st, v, mem st, transactions st).
+Definition update_current_vmid (st : state) (v : vmid) : state :=
+  (get_vm_states st, v, get_mem st, get_transactions st).
 
-Definition isPrimary (st : State) : bool :=
-  (currentVM st) =? 0.
+Definition is_primary (st : state) : bool :=
+  (get_current_vm st) =? 0.
 
-Definition isSecondary (st : State) : bool :=
-  negb (isPrimary st).
+Definition is_secondary (st : state) : bool :=
+  negb (is_primary st).
 
-Definition isValidPC (st : State) : option bool :=
-  w <- getReg st PC ;;;
-  w' <- addrOffset w 1 ;;;
-  Some (andb (checkAccessAddr st (currentVM st) w) (checkAccessAddr st (currentVM st) w')).
+Definition is_valid_PC (st : state) : option bool :=
+  w <- get_reg st PC ;;;
+  w' <- addr_offset w 1 ;;;
+  Some (andb (check_access_addr st (get_current_vm st) w) (check_access_addr st (get_current_vm st) w')).
 
-Definition simpleOptionStateUnpack (oldSt : State) (newSt : option State) : Conf :=
+Definition option_state_unpack (oldSt : state) (newSt : option state) : conf :=
   match newSt with
   | None => (FailI, oldSt)
   | Some s => (NextI, s)
   end.
 
-Definition MovHelperWord (s : State) (dst : RegName) (src : Word) : Conf * ControlMode :=
+Definition mov_word (s : state) (dst : reg_name) (src : word) : conf * control_mode :=
   let comp :=
-        s' <- updateGeneralReg s dst src ;;;
-        updateIncrPC s'
+        s' <- update_general_reg s dst src ;;;
+        update_incr_PC s'
     in
-    (simpleOptionStateUnpack s comp, NormalM).
+    (option_state_unpack s comp, NormalM).
 
-Definition MovHelperReg (s : State) (dst : RegName) (src : RegName) : Conf * ControlMode :=
+Definition mov_reg (s : state) (dst : reg_name) (src : reg_name) : conf * control_mode :=
   let comp :=
-      src' <- getReg s src ;;;
-      s'' <- updateGeneralReg s dst src' ;;;
-      updateIncrPC s''
+      src' <- get_reg s src ;;;
+      s'' <- update_general_reg s dst src' ;;;
+      update_incr_PC s''
     in
-  (simpleOptionStateUnpack s comp, NormalM).
+  (option_state_unpack s comp, NormalM).
 
-Definition LdrHelper (s : State) (dst : RegName) (src : RegName) : Conf * ControlMode :=
+Definition ldr (s : state) (dst : reg_name) (src : reg_name) : conf * control_mode :=
   let comp :=
-      src' <- getReg s src ;;;
-      v <- getMem s src' ;;;
-      m <- updateGeneralReg s dst v ;;;
-      updateIncrPC m
+      src' <- get_reg s src ;;;
+      v <- get_memory s src' ;;;
+      m <- update_general_reg s dst v ;;;
+      update_incr_PC m
   in
-  (simpleOptionStateUnpack s comp, NormalM).
+  (option_state_unpack s comp, NormalM).
 
-Definition StrHelper (s : State) (src : RegName) (dst : RegName) : Conf * ControlMode :=
+Definition str (s : state) (src : reg_name) (dst : reg_name) : conf * control_mode :=
   let comp :=
-      src' <- getReg s src ;;;
-      dst' <- getReg s dst ;;;
-      m <- updateMem s dst' src' ;;;
-      updateIncrPC m
+      src' <- get_reg s src ;;;
+      dst' <- get_reg s dst ;;;
+      m <- update_memory s dst' src' ;;;
+      update_incr_PC m
   in
-  (simpleOptionStateUnpack s comp, NormalM).
+  (option_state_unpack s comp, NormalM).
 
-Program Definition CmpHelperWord (s : State) (arg1 : RegName) (arg2 : Word) : Conf * ControlMode :=
+Program Definition cmp_word (s : state) (arg1 : reg_name) (arg2 : word) : conf * control_mode :=
   let comp :=
-      arg1' <- getReg s arg1 ;;;
+      arg1' <- get_reg s arg1 ;;;
       m <- match (nat_lt_dec (fin_to_nat arg1') (fin_to_nat arg2)) with
-           | left _ => updateSysReg s NZ (@nat_to_fin 1 WordSize _)
-           | right _ => updateSysReg s NZ (@nat_to_fin 0 WordSize _)
+           | left _ => update_sys_reg s NZ (@nat_to_fin 1 word_size _)
+           | right _ => update_sys_reg s NZ (@nat_to_fin 0 word_size _)
            end ;;;
-      updateIncrPC m       
+      update_incr_PC m       
   in
-  (simpleOptionStateUnpack s comp, NormalM).
+  (option_state_unpack s comp, NormalM).
 Next Obligation.
-  pose proof WordSizeAtLeast as G.
-  unfold WordSizeLowerBound in G.
+  pose proof word_size_at_least as G.
+  unfold word_size_lower_bound in G.
   lia.
 Qed.
 Next Obligation.
-  pose proof WordSizeAtLeast as G.
-  unfold WordSizeLowerBound in G.
+  pose proof word_size_at_least as G.
+  unfold word_size_lower_bound in G.
   lia.
 Qed.
 
-Program Definition CmpHelperReg (s : State) (arg1 : RegName) (arg2 : RegName) : Conf * ControlMode :=
+Program Definition cmp_reg (s : state) (arg1 : reg_name) (arg2 : reg_name) : conf * control_mode :=
   let comp :=
-      arg1' <- getReg s arg1 ;;;
-      arg2' <- getReg s arg2 ;;;
+      arg1' <- get_reg s arg1 ;;;
+      arg2' <- get_reg s arg2 ;;;
       m <- match (nat_lt_dec (fin_to_nat arg1') (fin_to_nat arg2')) with
-           | left _ => updateSysReg s NZ (@nat_to_fin 1 WordSize _)
-           | right _ => updateSysReg s NZ (@nat_to_fin 0 WordSize _)
+           | left _ => update_sys_reg s NZ (@nat_to_fin 1 word_size _)
+           | right _ => update_sys_reg s NZ (@nat_to_fin 0 word_size _)
            end ;;;
-      updateIncrPC m
+      update_incr_PC m
   in
-  (simpleOptionStateUnpack s comp, NormalM).
+  (option_state_unpack s comp, NormalM).
 Next Obligation.
-  pose proof WordSizeAtLeast as G.
-  unfold WordSizeLowerBound in G.
+  pose proof word_size_at_least as G.
+  unfold word_size_lower_bound in G.
   lia.
 Qed.
 Next Obligation.
-  pose proof WordSizeAtLeast as G.
-  unfold WordSizeLowerBound in G.
+  pose proof word_size_at_least as G.
+  unfold word_size_lower_bound in G.
   lia.
 Qed.
 
-Definition JnzHelper (s : State) (arg : RegName) : Conf * ControlMode :=
+Definition jnz (s : state) (arg : reg_name) : conf * control_mode :=
   let comp :=
-      arg' <- getReg s arg ;;;
-      nz <- getReg s NZ ;;;
+      arg' <- get_reg s arg ;;;
+      nz <- get_reg s NZ ;;;
       match (fin_to_nat nz) with
-      | 0 => updateSysReg s PC arg'
-      | _ => updateIncrPC s
+      | 0 => update_sys_reg s PC arg'
+      | _ => update_incr_PC s
       end
   in
-  (simpleOptionStateUnpack s comp, NormalM).
+  (option_state_unpack s comp, NormalM).
 
-Definition JmpHelper (s : State) (arg : RegName) : Conf * ControlMode :=
+Definition jmp (s : state) (arg : reg_name) : conf * control_mode :=
   let comp :=
-      arg' <- getReg s arg ;;;
-      updateSysReg s PC arg'
+      arg' <- get_reg s arg ;;;
+      update_sys_reg s PC arg'
   in
-  (simpleOptionStateUnpack s comp, NormalM).
+  (option_state_unpack s comp, NormalM).
 
-Definition FailHelper (s : State) : Conf * ControlMode :=
+Definition fail (s : state) : conf * control_mode :=
   (FailI, s, NormalM).
 
-Definition HaltHelper (s : State) : Conf * ControlMode :=
+Definition halt (s : state) : conf * control_mode :=
   (HaltI, s, NormalM).
 
-Program Definition RunHelper (s : State) : Conf * ControlMode :=
-  match getReg s  (R 1 _) with
+Program Definition run (s : state) : conf * control_mode :=
+  match get_reg s  (R 1 _) with
   | None => (FailI, s, NormalM)
   | Some id =>
-    match updateIncrPC s with
+    match update_incr_PC s with
     | None => (FailI, s, NormalM)
     | Some s' =>
-      match DecodeVMID id with
+      match decode_vmid id with
       | None => (FailI, s, NormalM)
       | Some id' => (NextI, s', YieldM id')
       end
     end
   end.
 Next Obligation.
-  pose proof RegCountAtLeast as G.
-  unfold RegCountLowerBound in G.
+  pose proof reg_count_at_least as G.
+  unfold reg_count_lower_bound in G.
   lia.
 Qed.
 
-Definition YieldHelper (s : State) : Conf * ControlMode :=
-  match updateIncrPC s with
+Program Definition sum_state_unpack (oldSt : state) (newSt : sum hvc_error state) : conf :=
+  match newSt with
+  | inl err =>
+    match (update_general_reg oldSt (R 0 _) (encode_hvc_error err)) with
+    | None => (FailI, oldSt)
+    | Some s => (NextI, s)
+    end
+  | inr s => (NextI, s)
+  end.
+Next Obligation.
+  pose proof reg_count_at_least as G.
+  unfold reg_count_lower_bound in G.
+  lia.
+Qed.
+
+Definition yield (s : state) : conf * control_mode :=
+  match update_incr_PC s with
   | None => (FailI, s, NormalM)
-  | Some s' => (NextI, s', YieldM (@nat_to_fin 0 VMCount VMCountPos))
+  | Some s' => (NextI, s', YieldM (@nat_to_fin 0 vm_count vm_count_pos))
   end.
 
-Definition verifyPermTransaction (s : State) (p : Perm) (td : TransactionDescriptor) : bool :=
+Definition verify_perm_transaction (s : state) (p : permission) (td : transaction_descriptor) : bool :=
   match td with
   | (_, _, _, _, m) => map_fold
-                         (fun _ v acc => andb acc (set_fold (fun v' acc' => andb acc' (checkPermPage s (currentVM s) v' p)) true v))
+                         (fun _ v acc => andb acc (set_fold (fun v' acc' => andb acc' (check_perm_page s (get_current_vm s) v' p)) true v))
                          true
                          m
   end.
 
-Program Definition ShareHelper (s : State) : Conf * ControlMode :=
+Program Definition share (s : state) : conf * control_mode :=
     let comp :=
-        r <- getReg s (R 1 _) ;;;
-        m <- (if (PageSize <? fin_to_nat r)
+        r <- get_reg s (R 1 _) ;;;
+        m <- (if (page_size <? fin_to_nat r)
               then None
               else
-                txBAddr <- getTXBaseAddrGlobal s (currentVM s) ;;;
-                td <- parseTransactionDescriptor s r txBAddr Sharing ;;;
-                if (verifyPermTransaction s (Owned, ExclusiveAccess) td)
-                then bind (newTransactionFromDescriptor s Sharing td) (fun x => Some (x, td))
+                txBAddr <- get_tx_base_addr_global s (get_current_vm s) ;;;
+                td <- parse_transaction_descriptor s r txBAddr Sharing ;;;
+                if (verify_perm_transaction s (Owned, ExclusiveAccess) td)
+                then bind (new_transaction_from_descriptor s Sharing td) (fun x => Some (x, td))
                 else None) ;;;
         match m with
-        | (m', td) => _
+        | (m', td) =>
+          match td with
+          | (_, gm) =>
+            match (map_fold (fun _ v acc => union v acc) empty gm) with
+            | ListsetNoDup ls prf =>
+              foldr (fun v' acc' => bind acc' (fun x => update_page_table x v' (Owned, SharedAccess))) (Some m') ls
+            end
+          end
         end
     in 
-    (simpleOptionStateUnpack s comp, NormalM).
+    (option_state_unpack s comp, NormalM).
 Next Obligation.
-  pose proof RegCountAtLeast as G.
-  unfold RegCountLowerBound in G.
+  pose proof reg_count_at_least as G.
+  unfold reg_count_lower_bound in G.
   lia.
 Defined.
-Next Obligation.
-  intros.
-  destruct td.
-  pose proof (map_fold (fun _ v acc => union v acc) empty g) as G.
-  destruct G as [ls prf].
-  exact (monad_general.foldrMList (fun v' acc' => updatePageTable acc' v' (Owned, SharedAccess)) ls m').
-Defined.
 
-Program Definition LendHelper (s : State) : Conf * ControlMode :=
+Program Definition lend (s : state) : conf * control_mode :=
   let comp :=
-      r <- getReg s (R 1 _) ;;;
-      m <- (if (PageSize <? fin_to_nat r)
+      r <- get_reg s (R 1 _) ;;;
+      m <- (if (page_size <? fin_to_nat r)
             then None
             else
-              txBAddr <- getTXBaseAddrGlobal s (currentVM s) ;;;
-              td <- parseTransactionDescriptor s r txBAddr Lending ;;;
-              if (verifyPermTransaction s (Owned, ExclusiveAccess) td)
-              then bind (newTransactionFromDescriptor s Lending td) (fun x => Some (x, td))
+              txBAddr <- get_tx_base_addr_global s (get_current_vm s) ;;;
+              td <- parse_transaction_descriptor s r txBAddr Lending ;;;
+              if (verify_perm_transaction s (Owned, ExclusiveAccess) td)
+              then bind (new_transaction_from_descriptor s Lending td) (fun x => Some (x, td))
               else None) ;;;
       match m with
-      | (m', td) => _
+      | (m', td) =>
+        match td with
+        | (_, gm) =>
+          match map_fold (fun _ v acc => union v acc) empty gm with
+          | ListsetNoDup ls prf =>
+            foldr (fun v' acc' => bind acc' (fun x => update_page_table x v' (Owned, NoAccess))) (Some m') ls
+          end
+        end
       end
   in 
-  (simpleOptionStateUnpack s comp, NormalM).
+  (option_state_unpack s comp, NormalM).
 Next Obligation.
-  pose proof RegCountAtLeast as G.
-  unfold RegCountLowerBound in G.
+  pose proof reg_count_at_least as G.
+  unfold reg_count_lower_bound in G.
   lia.
 Defined.
-Next Obligation.
-  intros.
-  destruct td.
-  pose proof (map_fold (fun _ v acc => union v acc) empty g) as G.
-  destruct G as [ls prf].
-  exact (monad_general.foldrMList (fun v' acc' => updatePageTable acc' v' (Owned, NoAccess)) ls m').
-Defined.
 
-Program Definition DonateHelper (s : State) : Conf * ControlMode :=
+Program Definition donate (s : state) : conf * control_mode :=
   let comp :=
-      r <- getReg s (R 1 _) ;;;
-      m <- (if (PageSize <? fin_to_nat r)
+      r <- get_reg s (R 1 _) ;;;
+      m <- (if (page_size <? fin_to_nat r)
             then None
             else
-              txBAddr <- getTXBaseAddrGlobal s (currentVM s) ;;;
-              td <- parseTransactionDescriptor s r txBAddr Donation ;;;
-              if (verifyPermTransaction s (Owned, ExclusiveAccess) td)
-              then bind (newTransactionFromDescriptor s Donation td) (fun x => Some (x, td))
+              txBAddr <- get_tx_base_addr_global s (get_current_vm s) ;;;
+              td <- parse_transaction_descriptor s r txBAddr Donation ;;;
+              if (verify_perm_transaction s (Owned, ExclusiveAccess) td)
+              then bind (new_transaction_from_descriptor s Donation td) (fun x => Some (x, td))
               else None) ;;;
       match m with
-      | (m', td) => _
+      | (m', td) =>
+        match td with
+        | (_, gm) =>
+          match map_fold (fun _ v acc => union v acc) empty gm with
+          | ListsetNoDup ls prf =>
+            foldr (fun v' acc' => bind acc' (fun x => update_page_table x v' (NotOwned, NoAccess))) (Some m') ls
+          end
+        end
       end
   in 
-  (simpleOptionStateUnpack s comp, NormalM).
+  (option_state_unpack s comp, NormalM).
 Next Obligation.
-  pose proof RegCountAtLeast as G.
-  unfold RegCountLowerBound in G.
+  pose proof reg_count_at_least as G.
+  unfold reg_count_lower_bound in G.
   lia.
 Defined.
-Next Obligation.
-  intros.
-  destruct td.
-  pose proof (map_fold (fun _ v acc => union v acc) empty g) as G.
-  destruct G as [ls prf].
-  exact (monad_general.foldrMList (fun v' acc' => updatePageTable acc' v' (NotOwned, NoAccess)) ls m').
-Defined.
 
-Definition toggleTransactionEntry (s : State) (h : Handle) (v : VMID) (p : PID) : State :=
-  (vmStates s, currentVM s, mem s,
+Definition toggle_transaction_entry (s : state) (h : handle) (v : vmid) (p : pid) : state :=
+  (get_vm_states s, get_current_vm s, get_mem s,
    alter (fun x => match x with
                    | (vs, w1, w2, gm, ty) => (vs, w1, w2, alter (fun y => alter (fun z => negb z) p y) v gm, ty)
-                   end) h (transactions s)).
+                   end) h (get_transactions s)).
 
-Program Definition toggleTransactionEntries (s : State) (h : Handle) (v : VMID) : State.
+Definition toggle_transaction_entries (s : state) (h : handle) (v : vmid) : state.
 Proof.
   intros.
-  destruct ((transactions s) !! h) as [[[? t] ?] |].
+  destruct ((get_transactions s) !! h) as [[[? t] ?] |].
   - destruct (t !! v) as [g |].
-    + exact (map_fold (fun k _ acc => toggleTransactionEntry acc h v k) s g).
+    + exact (map_fold (fun k _ acc => toggle_transaction_entry acc h v k) s g).
     + exact s.
   - exact s.
 Defined.
 
-Definition getPIDs (s : State) (handle : Handle) : list PID :=
-  match (transactions s) !! handle with
+Definition get_pids (s : state) (h : handle) : list pid :=
+  match (get_transactions s) !! h with
   | None => nil
   | Some (_, _, _, m, _) =>
-    match m !! (currentVM s) with
+    match m !! (get_current_vm s) with
     | None => nil
     | Some m' => map (fun x => match x with | (y, _) => y end) (map_to_list m')
     end
   end.
 
-Definition retrieveTransaction (s : State)
-           (handle : Handle)
-           (type : TransactionType)
-           (receiversMap : gmap VMID (gmap PID Flag)) : option State :=
+Definition retrieve_transaction (s : state)
+           (h : handle)
+           (type : transaction_type)
+           (receiversMap : gmap vmid (gmap pid bool)) : option state :=
+  let m := toggle_transaction_entries s h (get_current_vm s)
+  in
   match type with
   | Sharing =>
-    let m := toggleTransactionEntries s handle (currentVM s)
-    in (monad_general.foldrMList (fun v' acc' => updatePageTable acc' v' (NotOwned, SharedAccess)) (getPIDs s handle) m)
+    foldr (fun v' acc' =>
+             bind acc'
+                  (fun x => update_page_table x v' (NotOwned, SharedAccess)))
+          (Some m)
+          (get_pids s h)
   | Lending =>
-    let m := toggleTransactionEntries s handle (currentVM s)
-    in if decide (1 < size receiversMap)
-       then (monad_general.foldrMList (fun v' acc' => updatePageTable acc' v' (NotOwned, SharedAccess)) (getPIDs s handle) m)
-       else (monad_general.foldrMList (fun v' acc' => updatePageTable acc' v' (NotOwned, ExclusiveAccess)) (getPIDs s handle) m)
+    if decide (1 < size receiversMap)
+    then foldr (fun v' acc' =>
+                  bind acc' (fun x => update_page_table x v' (NotOwned, SharedAccess)))
+               (Some m)
+               (get_pids s h)
+    else foldr (fun v' acc' =>
+                  bind acc' (fun x => update_page_table x v' (NotOwned, ExclusiveAccess)))
+               (Some m)
+               (get_pids s h)
   | Donation =>
-    let m := toggleTransactionEntries s handle (currentVM s)
-    in (monad_general.foldrMList (fun v' acc' => updatePageTable acc' v' (Owned, ExclusiveAccess)) (getPIDs s handle) m)
+    foldr (fun v' acc' =>
+             bind acc' (fun x => update_page_table x v' (Owned, ExclusiveAccess)))
+          (Some m)
+          (get_pids s h)
   end.
 
-Definition relinquishTransaction (s : State)
-           (handle : Handle) : option State :=
-  let m := toggleTransactionEntries s handle (currentVM s)
-  in (monad_general.foldrMList (fun v' acc' => updatePageTable acc' v' (NotOwned, NoAccess)) (getPIDs s handle) m).
+Definition relinquish_transaction (s : state)
+           (h : handle) : option state :=
+  let m := toggle_transaction_entries s h (get_current_vm s)
+  in foldr (fun v' acc' => bind acc' (fun x => update_page_table x v' (NotOwned, NoAccess))) (Some m) (get_pids s h).
 
-Definition receivers (t : Transaction) : gmap VMID (gmap PID Flag) :=
+Definition get_receivers (t : transaction) : gmap vmid (gmap pid bool) :=
   match t with
   | (_, _, _, m, _) => m
   end.
 
-Definition type (t : Transaction) : TransactionType :=
+Definition get_type (t : transaction) : transaction_type :=
   match t with
   | (_, _, _, _, ty) => ty
   end.
 
-Program Definition RetrieveHelper (s : State) : Conf * ControlMode :=
+Program Definition retrieve (s : state) : conf * control_mode :=
   let comp :=
-      handle <- getReg s (R 1 _) ;;;
-      trn <- getTransaction s handle ;;;
-      m <- retrieveTransaction s handle (type trn) (receivers trn) ;;;
-      updateIncrPC m
+      handle <- get_reg s (R 1 _) ;;;
+      trn <- get_transaction s handle ;;;
+      m <- retrieve_transaction s handle (get_type trn) (get_receivers trn) ;;;
+      update_incr_PC m
   in
-  (simpleOptionStateUnpack s comp, NormalM).
+  (option_state_unpack s comp, NormalM).
 Next Obligation.
-  pose proof RegCountAtLeast as G.
-  unfold RegCountLowerBound in G.
+  pose proof reg_count_at_least as G.
+  unfold reg_count_lower_bound in G.
   lia.
 Defined.
 
-Program Definition RelinquishHelper (s : State) : Conf * ControlMode :=
+Program Definition relinquish (s : state) : conf * control_mode :=
   let comp :=
-      handle <- getReg s (R 1 _) ;;;
-      m <- relinquishTransaction s handle ;;;
-      updateIncrPC m
+      handle <- get_reg s (R 1 _) ;;;
+      m <- relinquish_transaction s handle ;;;
+      update_incr_PC m
   in
-  (simpleOptionStateUnpack s comp, NormalM).
+  (option_state_unpack s comp, NormalM).
 Next Obligation.
-  pose proof RegCountAtLeast as G.
-  unfold RegCountLowerBound in G.
+  pose proof reg_count_at_least as G.
+  unfold reg_count_lower_bound in G.
   lia.
 Defined.
 
-Definition allNotReceived (s : State) (handle : Handle) (v : VMID) : bool :=
-  match (transactions s) !! handle with
+Definition all_not_received (s : state) (h : handle) (v : vmid) : bool :=
+  match (get_transactions s) !! h with
   | None => true
   | Some (_, _, _, m, _) =>
     match m !! v with
@@ -872,87 +871,88 @@ Definition allNotReceived (s : State) (handle : Handle) (v : VMID) : bool :=
     end
   end.
 
-Program Definition ReclaimHelper (s : State) : Conf * ControlMode :=
+Program Definition reclaim (s : state) : conf * control_mode :=
   let comp :=
-      handle <- getReg s (R 1 _) ;;;
-      m <- (if allNotReceived s handle (currentVM s)
+      handle <- get_reg s (R 1 _) ;;;
+      m <- (if all_not_received s handle (get_current_vm s)
             then
-              (monad_general.foldrMList
-                 (fun v' acc' => updatePageTable acc' v' (Owned, ExclusiveAccess))
-                 (getPIDs s handle) (removeTransaction s handle))
+              foldr
+                (fun v' acc' => bind acc' (fun x => update_page_table x v' (Owned, ExclusiveAccess)))
+                                     (Some (remove_transaction s handle))
+                                     (get_pids s handle)
             else None) ;;;
-      updateIncrPC m
+      update_incr_PC m
   in
-  (simpleOptionStateUnpack s comp, NormalM).
+  (option_state_unpack s comp, NormalM).
 Next Obligation.
-  pose proof RegCountAtLeast as G.
-  unfold RegCountLowerBound in G.
+  pose proof reg_count_at_least as G.
+  unfold reg_count_lower_bound in G.
   lia.
 Defined.
 
-Program Definition SendHelper (s : State) : Conf * ControlMode :=
+Program Definition send (s : state) : conf * control_mode :=
   let comp :=
-      receiver <- getReg s (R 1 _) ;;;
-      receiver' <- DecodeVMID receiver ;;;
-      m <- transferMsgUnsafe s (currentVM s) receiver' ;;;
-      updateIncrPC m
+      receiver <- get_reg s (R 1 _) ;;;
+      receiver' <- decode_vmid receiver ;;;
+      m <- transfer_msg_unsafe s (get_current_vm s) receiver' ;;;
+      update_incr_PC m
   in
-  (simpleOptionStateUnpack s comp, NormalM).
+  (option_state_unpack s comp, NormalM).
 Next Obligation.
-  pose proof RegCountAtLeast as G.
-  unfold RegCountLowerBound in G.
+  pose proof reg_count_at_least as G.
+  unfold reg_count_lower_bound in G.
   lia.
 Defined.
 
-Definition WaitHelper (s : State) : Conf * ControlMode :=
-  match updateIncrPC s with
+Definition wait (s : state) : conf * control_mode :=
+  match update_incr_PC s with
   | None => (FailI, s, NormalM)
   | Some s' =>
-    if isRXReady s
+    if is_rx_ready s
     then (NextI, s', NormalM)
-    else (NextI, s', YieldM (@nat_to_fin 0 _ VMCountPos))
+    else (NextI, s', YieldM (@nat_to_fin 0 _ vm_count_pos))
   end.
 
-Program Definition HvcHelper (s : State) : Conf * ControlMode :=
-  match getReg s (R 0 _) with
-  | None => FailHelper s
+Program Definition hvc (s : state) : conf * control_mode :=
+  match get_reg s (R 0 _) with
+  | None => fail s
   | Some r0 =>
-    match DecodeHvcFunc r0 with
-    | None => FailHelper s
+    match decode_hvc_func r0 with
+    | None => fail s
     | Some func =>
       match func with
-      | Run => RunHelper s
-      | Yield => YieldHelper s
-      | Share => ShareHelper s
-      | Lend => LendHelper s
-      | Donate => DonateHelper s
-      | Retrieve => RetrieveHelper s
-      | Relinquish => RelinquishHelper s
-      | Reclaim => ReclaimHelper s
-      | Send => SendHelper s
-      | Wait => WaitHelper s
+      | Run => run s
+      | Yield => yield s
+      | Share => share s
+      | Lend => lend s
+      | Donate => donate s
+      | Retrieve => retrieve s
+      | Relinquish => relinquish s
+      | Reclaim => reclaim s
+      | Send => send s
+      | Wait => wait s
       end
     end
   end.
 Next Obligation.
-  pose proof RegCountAtLeast as G.
-  unfold RegCountLowerBound in G.
+  pose proof reg_count_at_least as G.
+  unfold reg_count_lower_bound in G.
   lia.
 Qed.
 
-Definition exec (i : Instruction) (s : State) : Conf * ControlMode :=
+Definition exec (i : instruction) (s : state) : conf * control_mode :=
   match i with
-  | Mov dst (inl srcWord) => MovHelperWord s dst srcWord
-  | Mov dst (inr srcReg) => MovHelperReg s dst srcReg
-  | Ldr dst src => LdrHelper s dst src
-  | Str src dst => StrHelper s src dst
-  | Cmp arg1 (inl arg2) => CmpHelperWord s arg1 arg2
-  | Cmp arg1 (inr arg2) => CmpHelperReg s arg1 arg2
-  | Jnz arg => JnzHelper s arg
-  | Jmp arg => JmpHelper s arg
-  | Fail => FailHelper s
-  | Halt => HaltHelper s
-  | Hvc => HvcHelper s
+  | Mov dst (inl srcWord) => mov_word s dst srcWord
+  | Mov dst (inr srcReg) => mov_reg s dst srcReg
+  | Ldr dst src => ldr s dst src
+  | Str src dst => str s src dst
+  | Cmp arg1 (inl arg2) => cmp_word s arg1 arg2
+  | Cmp arg1 (inr arg2) => cmp_reg s arg1 arg2
+  | Jnz arg => jnz s arg
+  | Jmp arg => jmp s arg
+  | Fail => fail s
+  | Halt => halt s
+  | Hvc => hvc s
   end.
 
 Inductive val : Type :=
@@ -961,7 +961,7 @@ Inductive val : Type :=
 | FailV.
 
 Inductive expr: Type :=
-| Instr (c : ExecMode)
+| Instr (c : exec_mode)
 | Seq (e : expr).
 
 Definition of_val (v : val) : expr :=
@@ -1003,49 +1003,26 @@ Definition fill_item (Ki : ectx_item) (e : expr) : expr :=
   | SeqCtx => Seq e
   end.
 
-Inductive step : Conf -> Conf * ControlMode -> Prop :=
+Inductive step : conf -> conf * control_mode -> Prop :=
 | step_exec_fail:
     forall st,
-      not (isValidPC st = Some true) ->
+      not (is_valid_PC st = Some true) ->
       step (ExecI, st) (FailI, st, NormalM)
 | step_exec_instr:
     forall st a w1 w2 i c,
-      isValidPC st = Some true ->
-      getReg st PC = Some a ->
-      getMem st a = Some w1 ->
-      getMemWithOffset st a 1 = Some w2 ->
-      DecodeInstr (w1, w2) = Some i ->
+      is_valid_PC st = Some true ->
+      get_reg st PC = Some a ->
+      get_memory st a = Some w1 ->
+      get_memory_with_offset st a 1 = Some w2 ->
+      decode_instruction (w1, w2) = Some i ->
       exec i st = c ->
       step (ExecI, st) c.
 
-Inductive prim_step : expr -> State -> list Empty_set -> expr -> State -> list Empty_set -> ControlMode -> Prop :=
+Inductive prim_step : expr -> state -> list Empty_set -> expr -> state -> list Empty_set -> control_mode -> Prop :=
 | PS_instr_normal st e' st' :
     step (ExecI, st) (e', st', NormalM) -> prim_step (Instr ExecI) st [] (Instr e') st' [] NormalM
 | PS_instr_yield st e' st' i :
-    step (ExecI, st) (e', st', YieldM i) -> prim_step (Instr ExecI) st [] (Instr e') (updateCurrentVMID st' i) [] NormalM
+    step (ExecI, st) (e', st', YieldM i) -> prim_step (Instr ExecI) st [] (Instr e') (update_current_vmid st' i) [] NormalM
 | PS_seq st : prim_step (Seq (Instr NextI)) st [] (Seq (Instr ExecI)) st [] NormalM
 | PS_halt st : prim_step (Seq (Instr HaltI)) st [] (Instr HaltI) st [] NormalM
 | PS__fail st : prim_step (Seq (Instr FailI)) st [] (Instr FailI) st [] NormalM.
-
-(*
-Lemma fill_item_val Ki e :
-    is_Some (to_val (fill_item Ki e)) → is_Some (to_val e).
-Proof.
-  intros [v ?]. destruct Ki; simplify_option_eq; eauto.
-Qed.
-
-Instance fill_item_inj Ki : Inj (=) (=) (fill_item Ki).
-Proof.
-  destruct Ki; intros ???; simplify_eq; auto with f_equal.
-Qed.
-
-Lemma fill_item_no_val_inj Ki1 Ki2 e1 e2 :
-  to_val e1 = None → to_val e2 = None →
-  fill_item Ki1 e1 = fill_item Ki2 e2 → Ki1 = Ki2.
-Proof.
-  destruct Ki1, Ki2; intros; try discriminate; simplify_eq;
-    repeat match goal with
-           | HH : to_val (of_val _) = None |- _ => by rewrite to_of_val in HH
-           end; auto.
-Qed.
-*)
